\documentclass{article}
\usepackage{amsmath}
\usepackage{array}
\usepackage[margin=0.5in]{geometry}  % Set all margins to 0.5 inch

% Remove extra space around section headers
\usepackage{titlesec}
\titlespacing*{\section}{0pt}{12pt}{6pt}
\titlespacing*{\subsection}{0pt}{12pt}{6pt}

% Adjust equation spacing
\setlength{\abovedisplayskip}{6pt}
\setlength{\belowdisplayskip}{6pt}
\setlength{\abovedisplayshortskip}{3pt}
\setlength{\belowdisplayshortskip}{3pt}

\begin{document}

\section*{Consistent system with infinitely many solutions}
\vspace{1em}

Consider the augmented matrix:
\[
\begin{bmatrix}
1 & 0 & -5 & | & 1 \\
0 & 1 & \frac{1}{2} & | & 4 \\
0 & 0 & 0 & | & 0
\end{bmatrix}
\]

This system reduces to:
\begin{align*}
x_1 - 5x_3 &= 1 \\
x_2 + x_3 &= 4 \\
0 &= 0
\end{align*}

Solving for $x_1$ and $x_2$ in terms of $x_3$:
\[
\begin{cases}
x_1 = 5x_3 + 1 \\
x_2 = 4 - x_3 \\
x_3 \text{ is free}
\end{cases}
\]

\textbf{Note:} Free variables can take on any value. Once you choose a value for your free variable, it will determine the values of the other (basic) variables.

\textbf{Example Solutions:}

When $x_3 = 2$:
\begin{align*}
x_1 &= 5(2) + 1 = 10 + 1 = 11 \\
x_2 &= 4 - 2 = 2
\end{align*}
Solution point: $(11, 2, 2)$

When $x_3 = -6$:
\begin{align*}
x_1 &= 5(-6) + 1 = -30 + 1 = -29 \\
x_2 &= 4 + 6 = 10
\end{align*}
Solution point: $(-29, 10, -6)$

\section*{Example: Inconsistent System}
Consider the system:
\begin{align*}
x_1 - 2x_2 - x_3 + 3x_4 &= 0 \\
-2x_1 + 4x_2 + 5x_3 - 5x_4 &= 3 \\
3x_1 - 6x_2 - 6x_3 + 8x_4 &= 2
\end{align*}

The augmented matrix reduces to:
\[
\begin{bmatrix}
1 & -2 & -1 & 3 & | & 0 \\
0 & 0 & 3 & 1 & | & 3 \\
0 & 0 & -3 & -1 & | & 2
\end{bmatrix}
\rightarrow
\begin{bmatrix}
1 & -2 & -1 & 3 & | & 0 \\
0 & 0 & 0 & 0 & | & 5 \\
0 & 0 & -3 & -1 & | & 2
\end{bmatrix}
\]

This system is inconsistent because the row $[0 \; 0 \; 0 \; 0 \; | \; 5]$ implies $0 = 5$.

\section*{Practice: System with Free Variable}
Given the augmented matrix:
\[
\begin{bmatrix}
1 & 3 & 4 & | & 7 \\
3 & 9 & 7 & | & 6
\end{bmatrix}
\]

After row reduction:
\[
\begin{bmatrix}
1 & 3 & 4 & | & 7 \\
0 & 0 & 1 & | & 3
\end{bmatrix}
\]

From this, we get:
\begin{align*}
x_1 + 3x_2 + 4x_3 &= 7 \\
x_3 &= 3
\end{align*}

Substituting $x_3 = 3$:
\begin{align*}
x_1 + 3x_2 + 4(3) &= 7 \\
x_1 + 3x_2 + 12 &= 7 \\
x_1 + 3x_2 &= -5 \\
x_1 &= -5 - 3x_2
\end{align*}

The general solution is:
\[
\begin{cases}
x_1 = -5 - 3x_2 \\
x_2 \text{ is free} \\
x_3 = 3
\end{cases}
\]

\end{document}